Closed example of distributed composition for bank

src/program_proof/memkv/closed.v
@@ -1,9 +1,10 @@
+From Perennial.algebra Require Import auth_map.
 From Perennial.algebra Require Import gen_heap_names.
 From Perennial.goose_lang Require Import lang notation typing lifting.
 From Perennial.goose_lang.lib Require Import map.impl list.impl list_slice.
 From Perennial.goose_lang Require Import prelude.
 From Perennial.goose_lang Require Import ffi.grove_prelude.
-From Goose.github_com.mit_pdos.gokv Require Import memkv connman.
+From Goose.github_com.mit_pdos.gokv Require Import memkv connman bank.
 
 
 From Perennial.program_proof Require Import grove_prelude.
@@ -12,7 +13,12 @@ From Perennial.program_proof.memkv Require Export
      memkv_shard_definitions memkv_shard_start_proof memkv_shard_make_proof memkv_shard_ghost_init.
 From Perennial.program_proof.memkv Require Export
      memkv_coord_definitions memkv_coord_start_proof memkv_coord_make_proof memkv_coord_ghost_init.
-From Perennial.program_proof.memkv Require Export memkv_clerk_proof.
+From Perennial.program_proof.memkv Require Export memkv_clerk_proof bank_proof.
+
+From Perennial.goose_lang Require adequacy dist_adequacy.
+From Perennial.goose_lang.ffi Require grove_ffi_adequacy.
+
+Module closed1.
 
 Definition shard_boot (host : u64) : expr :=
   let: "s" := MakeKVShardServer #true in
@@ -26,8 +32,7 @@ Definition client_boot (coord : u64) : expr :=
   let: "cm" := MakeConnMan #() in
   MakeKVClerk #coord "cm".
 
-From Perennial.goose_lang Require Import adequacy dist_adequacy grove_ffi_adequacy.
-From Perennial.goose_lang.ffi Require Import grove_ffi_adequacy.
+Import adequacy dist_adequacy grove_ffi_adequacy.
 
 Definition shardΣ := #[heapΣ; kvMapΣ; rpcΣ ShardReplyC; rpcregΣ].
 
@@ -139,3 +144,276 @@ Proof.
     eauto.
   }
 Qed.
+
+End closed1.
+
+Module closed2.
+
+Definition shard_boot (host : u64) : expr :=
+  let: "s" := MakeKVShardServer #true in
+  KVShardServer__Start "s" #host.
+
+Definition coord_boot (host : u64) (init : u64) : expr :=
+  let: "s" := MakeKVCoordServer #init in
+  KVCoord__Start "s" #host.
+
+Definition transferrer_boot (lockcoord kvcoord : u64) (init acc1 acc2 : u64)  : expr :=
+  let: "cm" := MakeConnMan #() in
+  let: "ck" := MakeBankClerk #lockcoord #kvcoord "cm" #init #acc1 #acc2 #0 in
+  BankClerk__SimpleTransfer "ck" #1.
+
+Definition auditor_boot (lockcoord kvcoord : u64) (init acc1 acc2 : u64)  : expr :=
+  let: "cm" := MakeConnMan #() in
+  let: "ck" := MakeBankClerk #lockcoord #kvcoord "cm" #init #acc1 #acc2 #0 in
+  BankClerk__SimpleAudit "ck".
+
+Import adequacy dist_adequacy grove_ffi_adequacy.
+
+Definition shardΣ := #[heapΣ; kvMapΣ; rpcΣ ShardReplyC; rpcregΣ; mapΣ u64 u64].
+
+(* TODO: move *)
+Lemma heapG_heap_globalG_roundtrip {Σ} Hheap Hcrash local_names :
+  Hheap =
+  @heapG_heap_globalG Σ
+    (@dist_heapGS_heapGS grove_op grove_model grove_semantics grove_interp grove_interp_adequacy Σ Hheap
+       Hcrash local_names).
+Proof.
+  rewrite /heapG_heap_globalG. rewrite /dist_heapGS_heapGS //=.
+  destruct Hheap => //=. f_equal.
+  * destruct dist_heapGpreS => //= . f_equal.
+    { destruct heap_preG_iris => //=. }
+    { destruct heap_preG_crash => //=. }
+    { destruct heap_preG_heap => //=. }
+    { destruct heap_preG_ffi => //=. }
+    { destruct heap_preG_trace => //=. }
+    { destruct heap_preG_credit => //=. }
+  * rewrite gen_heapG_update_pre_get //=.
+  * rewrite /inv_get_names //=.
+    destruct dist_heapGS_inv_names => //=.
+Qed.
+
+Definition lockshardId := U64 0.
+Definition lockcoordId := U64 1.
+Definition kvshardId := U64 2.
+Definition kvcoordId := U64 3.
+
+Definition init := U64 0.
+Definition acc1 := U64 1.
+Definition acc2 := U64 2.
+
+Lemma bank_boot σlockshard σlockcoord σkvshard σkvcoord σclient (g : ffi_global_state) :
+  ffi_initgP g →
+  ffi_initP σlockshard.(world) g →
+  ffi_initP σlockcoord.(world) g →
+  ffi_initP σkvshard.(world) g →
+  ffi_initP σkvcoord.(world) g →
+  ffi_initP σclient.(world) g →
+  (g : gmap chan (gset message)) !! lockshardId = Some (∅ : gset message) →
+  (g : gmap chan (gset message)) !! lockcoordId = Some (∅ : gset message) →
+  (g : gmap chan (gset message)) !! kvshardId = Some (∅ : gset message) →
+  (g : gmap chan (gset message)) !! kvcoordId = Some (∅ : gset message) →
+  dist_adequate_failstop [
+                          (shard_boot lockshardId, σlockshard);
+                          (coord_boot lockcoordId lockshardId, σlockcoord);
+                          (shard_boot kvshardId, σkvshard);
+                          (coord_boot kvcoordId kvshardId, σkvcoord);
+                          (transferrer_boot lockcoordId kvcoordId init acc1 acc2, σclient);
+                          (auditor_boot lockcoordId kvcoordId init acc1 acc2, σclient)] g (λ _, True).
+Proof.
+  intros Hinitg
+         Hinitlockshard Hinitlockcoord
+         Hinitkvshard Hinitkvcoord
+         Hinitclient Hlookup1 Hlookup2 Hlookup3 Hlookup4.
+  eapply (grove_ffi_dist_adequacy_failstop (shardΣ)).
+  { assumption. }
+  intros Hheap.
+  iIntros "Hchan".
+
+  (* Init the channel inv for the lock shard server *)
+  iDestruct (big_sepM_delete with "Hchan") as "(Hlockshard_chan&Hrest)"; first eapply Hlookup1.
+  remember (uNSHARD) as uNSHARD' eqn:Heq_unSHARD'.
+  iMod (kvptsto_init uNSHARD') as (γlk) "(Hserver_lockshards&Hclients_lockptstos)"; first done.
+  iMod (shard_server_ghost_init lockshardId γlk with "[$Hlockshard_chan]")
+    as (γlk_shard Heq_lockshard) "(#Hdom&#Hsrv&Hsrv_rpc_ghost&Hsrv_cid)".
+
+  (* Init the channel inv for the lock coord server *)
+  iDestruct (big_sepM_delete with "Hrest") as "(Hlockcoord_chan&Hrest)".
+  { rewrite lookup_delete_ne; first eapply Hlookup2; eauto. }
+  iMod (coord_server_ghost_init lockcoordId γlk with "[$Hlockcoord_chan]")
+    as (γlk_coord Heq_lockcoord) "(#Hdom'&#Hsrv')".
+
+  (* Init the channel inv for the kv shard server *)
+  iDestruct (big_sepM_delete with "Hrest") as "(Hkvshard_chan&Hrest)".
+  { rewrite ?lookup_delete_ne; first eapply Hlookup3; eauto. }
+  iMod (kvptsto_init uNSHARD') as (γkv) "(Hserver_kvshards&Hclients_kvptstos)"; first done.
+  iMod (shard_server_ghost_init kvshardId γkv with "[$Hkvshard_chan]")
+    as (γkv_shard Heq_kvshard) "(#Hdom''&#Hsrv_kv&Hsrv_kv_rpc_ghost&Hsrv_kv_cid)".
+
+  (* Init the channel inv for the kv coord server *)
+  iDestruct (big_sepM_delete with "Hrest") as "(Hkvcoord_chan&_)".
+  { rewrite ?lookup_delete_ne; first eapply Hlookup4; eauto. }
+  iMod (coord_server_ghost_init kvcoordId γkv with "[$Hkvcoord_chan]")
+    as (γkv_coord Heq_kvcoord) "(#Hdom'''&#Hsrv'')".
+
+  (* Initialize the lock invariant for the init flag lock *)
+  (* Pull out the kv pts tos *)
+  iDestruct (big_sepS_delete _ _ init with "Hclients_kvptstos") as "(Hinit&Hclients_kvptstos)".
+  { apply elem_of_fin_to_set. }
+  iDestruct (big_sepS_delete _ _ acc1 with "Hclients_kvptstos") as "(Hacc1&Hclients_kvptstos)".
+  { set_unfold. eauto. }
+  iDestruct (big_sepS_delete _ _ acc2 with "Hclients_kvptstos") as "(Hacc2&Hclients_kvptstos)".
+  { set_unfold. eauto. }
+
+  (* Pull out the lock pts tos *)
+  iDestruct (big_sepS_delete _ _ init with "Hclients_lockptstos") as "(Hinit_lock&Hclients_lockptstos)".
+  { apply elem_of_fin_to_set. }
+  iDestruct (big_sepS_delete _ _ acc1 with "Hclients_lockptstos") as "(Hacc1_lock&Hclients_lockptstos)".
+  { set_unfold. eauto. }
+  iDestruct (big_sepS_delete _ _ acc2 with "Hclients_lockptstos") as "(Hacc2_lock&Hclients_lockptstos)".
+  { set_unfold. eauto. }
+
+  (* Finally alloc lock *)
+  iMod (lock_alloc lockN ⊤ _ init (init_lock_inv init acc1 acc2 _ _) with
+            "[$] [Hinit Hacc1 Hacc2 Hacc1_lock Hacc2_lock]") as "#His_lock".
+  { iLeft. iFrame "Hinit". iFrame. }
+
+  iSplitR ""; last first.
+  { iModIntro. iMod (fupd_mask_subseteq ∅); eauto. }
+
+  iModIntro.
+
+  (* lockserver shard *)
+  iSplitL "Hserver_lockshards Hsrv_rpc_ghost Hsrv_cid".
+  {
+    iIntros (Hcrash local_names).
+    iModIntro. iExists (λ _, True%I).
+    rewrite /shard_boot. simpl.
+    wp_bind (MakeKVShardServer #true).
+    wp_apply (wp_MakeKVShardServer with "[Hsrv_cid Hserver_lockshards Hsrv_rpc_ghost]").
+    { iSplitL "".
+      { rewrite is_shard_server_unfold. iNamed "Hsrv". iFrame "#". }
+      iClear "Hsrv". iFrame "Hsrv_rpc_ghost".
+      rewrite -Heq_unSHARD' Heq_lockshard. iFrame "Hserver_lockshards".
+      eauto. }
+    iIntros (s) "His_server".
+    wp_pures.
+    wp_apply (wp_KVShardServer__Start with "[] [] [$His_server]").
+    { iExactEq "Hdom". rewrite //=. f_equal. set_solver. }
+    { iExactEq "Hsrv". f_equal. apply heapG_heap_globalG_roundtrip. }
+    eauto.
+  }
+
+  (* lockserver coordinator *)
+  iSplitL "".
+  {
+    iIntros (Hcrash local_names).
+    iModIntro. iExists (λ _, True%I).
+    rewrite /coord_boot. simpl.
+    wp_bind (MakeKVCoordServer #(lockshardId : u64)).
+    wp_apply (wp_MakeKVCoordServer with "[]").
+    { iSplitL ""; last first.
+      { rewrite /named. iExactEq "Hsrv".
+        f_equal. apply heapG_heap_globalG_roundtrip. }
+      { iPureIntro. rewrite Heq_lockshard; symmetry; eauto. }
+    }
+    iIntros (s) "His_server".
+    wp_pures.
+    wp_apply (wp_KVCoordServer__Start with "[] [] [His_server]").
+    { iExactEq "Hdom'". rewrite //=. f_equal. set_solver. }
+    { iExactEq "Hsrv'". rewrite -heapG_heap_globalG_roundtrip. eauto. }
+    { iFrame "His_server". }
+    eauto.
+  }
+
+  (* kv shard *)
+  iSplitL "Hserver_kvshards Hsrv_kv_rpc_ghost Hsrv_kv_cid".
+  {
+    iIntros (Hcrash local_names).
+    iModIntro. iExists (λ _, True%I).
+    rewrite /shard_boot. simpl.
+    wp_bind (MakeKVShardServer #true).
+    wp_apply (wp_MakeKVShardServer with "[Hsrv_kv_cid Hserver_kvshards Hsrv_kv_rpc_ghost]").
+    { iSplitL "".
+      { iEval (rewrite is_shard_server_unfold) in "Hsrv_kv". iNamed "Hsrv_kv". iFrame "#". }
+      iClear "Hsrv". iFrame "Hsrv_kv_rpc_ghost".
+      rewrite -Heq_unSHARD' Heq_kvshard. iFrame "Hserver_kvshards".
+      eauto. }
+    iIntros (s) "His_server".
+    wp_pures.
+    wp_apply (wp_KVShardServer__Start with "[] [] [$His_server]").
+    { iExactEq "Hdom''". rewrite //=. f_equal. set_solver. }
+    { iExactEq "Hsrv_kv". f_equal. apply heapG_heap_globalG_roundtrip. }
+    eauto.
+  }
+
+  (* kv coordinator *)
+  iSplitL "".
+  {
+    iIntros (Hcrash local_names).
+    iModIntro. iExists (λ _, True%I).
+    rewrite /coord_boot. simpl.
+    wp_bind (MakeKVCoordServer #(kvshardId : u64)).
+    wp_apply (wp_MakeKVCoordServer with "[]").
+    { iSplitL ""; last first.
+      { rewrite /named. iExactEq "Hsrv_kv".
+        f_equal. apply heapG_heap_globalG_roundtrip. }
+      { iPureIntro. rewrite Heq_kvshard; symmetry; eauto. }
+    }
+    iIntros (s) "His_server".
+    wp_pures.
+    wp_apply (wp_KVCoordServer__Start with "[] [] [His_server]").
+    { iExactEq "Hdom'''". rewrite //=. f_equal. set_solver. }
+    { iExactEq "Hsrv''". rewrite -heapG_heap_globalG_roundtrip. eauto. }
+    { iFrame "His_server". }
+    eauto.
+  }
+
+  iSplitR "".
+  {
+    iIntros (Hcrash local_names).
+    iModIntro. iExists (λ _, True%I).
+    rewrite /transferrer_boot. iEval simpl.
+    wp_apply wp_MakeConnMan.
+    iIntros (cm) "Hcm".
+    wp_pures.
+    wp_apply (wp_MakeBankClerk with "[Hcm]").
+    { eauto. }
+    {
+      iSplitL "".
+      { iExactEq "Hsrv'". rewrite -heapG_heap_globalG_roundtrip. f_equal. }
+      iSplitL "".
+      { iExactEq "Hsrv''". rewrite -heapG_heap_globalG_roundtrip. f_equal. }
+      iFrame "Hcm". iExactEq "His_lock".
+      rewrite Heq_kvcoord Heq_lockcoord; auto.
+    }
+    iIntros (??) "(?&?)". wp_pures.
+    wp_apply (Bank__SimpleTransfer_spec with "[$]").
+    eauto.
+  }
+
+  iSplitR "".
+  {
+    iIntros (Hcrash local_names).
+    iModIntro. iExists (λ _, True%I).
+    rewrite /auditor_boot. iEval simpl.
+    wp_apply wp_MakeConnMan.
+    iIntros (cm) "Hcm".
+    wp_pures.
+    wp_apply (wp_MakeBankClerk with "[Hcm]").
+    { eauto. }
+    {
+      iSplitL "".
+      { iExactEq "Hsrv'". rewrite -heapG_heap_globalG_roundtrip. f_equal. }
+      iSplitL "".
+      { iExactEq "Hsrv''". rewrite -heapG_heap_globalG_roundtrip. f_equal. }
+      iFrame "Hcm". iExactEq "His_lock".
+      rewrite Heq_kvcoord Heq_lockcoord; auto.
+    }
+    iIntros (??) "(?&?)". wp_pures.
+    wp_apply (Bank__SimpleAudit_spec with "[$]").
+    eauto.
+  }
+  eauto.
+Qed.
+
+End closed2.
