src/program_proof/memkv/print_assumptions.v
@@ -1,9 +1,13 @@
 From Perennial.program_proof Require Import proof_prelude.
 From Perennial.program_proof.memkv Require Import closed memkv_clerk_proof.
 
-(* Closed proof for shard + coord server *)
-Print Assumptions shard_coord_boot.
-
-(* Client proofs -- not yet closed *)
-Definition client_theorems := (@KVClerk__Get, @KVClerk__MGet, @KVClerk__Put, @KVClerk__ConditionalPut).
+(* Client function wps *)
+Definition client_theorems := (@wp_KVClerk__Get, @wp_KVClerk__MGet, @wp_KVClerk__Put, @wp_KVClerk__ConditionalPut).
 Print Assumptions client_theorems.
+
+(* Closed proof for shard + coord server *)
+Print Assumptions closed1.shard_coord_boot.
+
+(* Closed proof for bank boot *)
+Print Assumptions closed2.bank_boot.
+
